Flapjack.lean
@@ -3,6 +3,7 @@ import Flapjack.PanSimp
 import Flapjack.PanStructs
 import Flapjack.PanGlobals
 import Flapjack.Pipeline
+import Flapjack.Correctness
 import Flapjack.Tests
 import Flapjack.Static
 import Flapjack.Crepe
